tuned names

src/HOL/Data_Structures/Height_Balanced_Tree.thy
@@ -20,8 +20,8 @@ definition empty :: "'a tree_ht" where
 text \<open>The maximal amount by which the height of two siblings may differ:\<close>
 
 locale HBT =
-fixes m :: nat
-assumes [arith]: "m > 0"
+fixes d :: nat
+assumes [arith]: "d > 0"
 begin
 
 text \<open>Invariant:\<close>
@@ -29,7 +29,7 @@ text \<open>Invariant:\<close>
 fun hbt :: "'a tree_ht \<Rightarrow> bool" where
 "hbt Leaf = True" |
 "hbt (Node l (a,n) r) =
- (abs(int(height l) - int(height r)) \<le> int(m) \<and>
+ (abs(int(height l) - int(height r)) \<le> int(d) \<and>
   n = max (height l) (height r) + 1 \<and> hbt l \<and> hbt r)"
 
 fun ht :: "'a tree_ht \<Rightarrow> nat" where
@@ -41,7 +41,7 @@ definition node :: "'a tree_ht \<Rightarrow> 'a \<Rightarrow> 'a tree_ht \<Right
 
 definition balL :: "'a tree_ht \<Rightarrow> 'a \<Rightarrow> 'a tree_ht \<Rightarrow> 'a tree_ht" where
 "balL AB b C =
-  (if ht AB = ht C + m + 1 then
+  (if ht AB = ht C + d + 1 then
      case AB of 
        Node A (a, _) B \<Rightarrow>
          if ht A \<ge> ht B then node A a (node B b C)
@@ -52,7 +52,7 @@ definition balL :: "'a tree_ht \<Rightarrow> 'a \<Rightarrow> 'a tree_ht \<Right
 
 definition balR :: "'a tree_ht \<Rightarrow> 'a \<Rightarrow> 'a tree_ht \<Rightarrow> 'a tree_ht" where
 "balR A a BC =
-   (if ht BC = ht A + m + 1 then
+   (if ht BC = ht A + d + 1 then
       case BC of
         Node B (b, _) C \<Rightarrow>
           if ht B \<le> ht C then node (node A a B) b C
@@ -130,34 +130,34 @@ by (cases t rule: tree2_cases) simp_all
 text \<open>First, a fast but relatively manual proof with many lemmas:\<close>
 
 lemma height_balL:
-  "\<lbrakk> hbt l; hbt r; height l = height r + m + 1 \<rbrakk> \<Longrightarrow>
-   height (balL l a r) \<in> {height r + m + 1, height r + m + 2}"
+  "\<lbrakk> hbt l; hbt r; height l = height r + d + 1 \<rbrakk> \<Longrightarrow>
+   height (balL l a r) \<in> {height r + d + 1, height r + d + 2}"
 by (auto simp:node_def balL_def split:tree.split)
 
 lemma height_balR:
-  "\<lbrakk> hbt l; hbt r; height r = height l + m + 1 \<rbrakk> \<Longrightarrow>
-   height (balR l a r) \<in> {height l + m + 1, height l + m + 2}"
+  "\<lbrakk> hbt l; hbt r; height r = height l + d + 1 \<rbrakk> \<Longrightarrow>
+   height (balR l a r) \<in> {height l + d + 1, height l + d + 2}"
 by(auto simp add:node_def balR_def split:tree.split)
 
 lemma height_node[simp]: "height(node l a r) = max (height l) (height r) + 1"
 by (simp add: node_def)
 
 lemma height_balL2:
-  "\<lbrakk> hbt l; hbt r; height l \<noteq> height r + m + 1 \<rbrakk> \<Longrightarrow>
+  "\<lbrakk> hbt l; hbt r; height l \<noteq> height r + d + 1 \<rbrakk> \<Longrightarrow>
    height (balL l a r) = 1 + max (height l) (height r)"
 by (simp_all add: balL_def)
 
 lemma height_balR2:
-  "\<lbrakk> hbt l;  hbt r;  height r \<noteq> height l + m + 1 \<rbrakk> \<Longrightarrow>
+  "\<lbrakk> hbt l;  hbt r;  height r \<noteq> height l + d + 1 \<rbrakk> \<Longrightarrow>
    height (balR l a r) = 1 + max (height l) (height r)"
 by (simp_all add: balR_def)
 
 lemma hbt_balL: 
-  "\<lbrakk> hbt l; hbt r; height r - m \<le> height l \<and> height l \<le> height r + m + 1 \<rbrakk> \<Longrightarrow> hbt(balL l a r)"
+  "\<lbrakk> hbt l; hbt r; height r - d \<le> height l \<and> height l \<le> height r + d + 1 \<rbrakk> \<Longrightarrow> hbt(balL l a r)"
 by(auto simp: balL_def node_def max_def split!: if_splits tree.split)
 
 lemma hbt_balR: 
-  "\<lbrakk> hbt l; hbt r; height l - m \<le> height r \<and> height r \<le> height l + m + 1 \<rbrakk> \<Longrightarrow> hbt(balR l a r)"
+  "\<lbrakk> hbt l; hbt r; height l - d \<le> height r \<and> height r \<le> height l + d + 1 \<rbrakk> \<Longrightarrow> hbt(balR l a r)"
 by(auto simp: balR_def node_def max_def split!: if_splits tree.split)
 
 text\<open>Insertion maintains @{const hbt}. Requires simultaneous proof.\<close>
@@ -190,12 +190,12 @@ proof (induction t rule: tree2_induct)
     proof(cases "x<a")
       case True
       show ?thesis
-      proof(cases "height (insert x l) = height r + m + 1")
+      proof(cases "height (insert x l) = height r + d + 1")
         case False with 2 Node(1,2) \<open>x < a\<close> show ?thesis by (auto simp: height_balL2)
       next
         case True 
-        hence "(height (balL (insert x l) a r) = height r + m + 1) \<or>
-          (height (balL (insert x l) a r) = height r + m + 2)" (is "?A \<or> ?B")
+        hence "(height (balL (insert x l) a r) = height r + d + 1) \<or>
+          (height (balL (insert x l) a r) = height r + d + 2)" (is "?A \<or> ?B")
           using 2 Node(1,2) height_balL[OF _ _ True] by simp
         thus ?thesis
         proof
@@ -207,12 +207,12 @@ proof (induction t rule: tree2_induct)
     next
       case False
       show ?thesis 
-      proof(cases "height (insert x r) = height l + m + 1")
+      proof(cases "height (insert x r) = height l + d + 1")
         case False with 2 Node(3,4) \<open>\<not>x < a\<close> show ?thesis by (auto simp: height_balR2)
       next
         case True 
-        hence "(height (balR l a (insert x r)) = height l + m + 1) \<or>
-          (height (balR l a (insert x r)) = height l + m + 2)"  (is "?A \<or> ?B")
+        hence "(height (balR l a (insert x r)) = height l + d + 1) \<or>
+          (height (balR l a (insert x r)) = height l + d + 2)"  (is "?A \<or> ?B")
           using Node 2 height_balR[OF _ _ True] by simp
         thus ?thesis 
         proof
@@ -265,12 +265,12 @@ proof (induct t rule: tree2_induct)
     proof(cases "x<a")
       case True
       show ?thesis
-      proof(cases "height r = height (delete x l) + m + 1")
+      proof(cases "height r = height (delete x l) + d + 1")
         case False with Node 1 \<open>x < a\<close> show ?thesis by(auto simp: balR_def)
       next
         case True 
-        hence "(height (balR (delete x l) a r) = height (delete x l) + m + 1) \<or>
-          height (balR (delete x l) a r) = height (delete x l) + m + 2" (is "?A \<or> ?B")
+        hence "(height (balR (delete x l) a r) = height (delete x l) + d + 1) \<or>
+          height (balR (delete x l) a r) = height (delete x l) + d + 2" (is "?A \<or> ?B")
           using Node 2height_balR[OF _ _ True] by simp
         thus ?thesis 
         proof
@@ -282,12 +282,12 @@ proof (induct t rule: tree2_induct)
     next
       case False
       show ?thesis
-      proof(cases "height l = height (delete x r) + m + 1")
+      proof(cases "height l = height (delete x r) + d + 1")
         case False with Node 1 \<open>\<not>x < a\<close> \<open>x \<noteq> a\<close> show ?thesis by(auto simp: balL_def)
       next
         case True 
-        hence "(height (balL l a (delete x r)) = height (delete x r) + m + 1) \<or>
-          height (balL l a (delete x r)) = height (delete x r) + m + 2" (is "?A \<or> ?B")
+        hence "(height (balL l a (delete x r)) = height (delete x r) + d + 1) \<or>
+          height (balL l a (delete x r)) = height (delete x r) + d + 2" (is "?A \<or> ?B")
           using Node 2 height_balL[OF _ _ True] by simp
         thus ?thesis 
         proof
